theories/typing/int.v
@@ -215,24 +215,19 @@ Section programs.
   Proof.
     move => Hnonneg Hsign Htestbit.
     rewrite /elem_of /int_elem_of_it /min_int /max_int.
+    have ? := bits_per_int_gt_0 it.
     destruct (it_signed it).
     - rewrite /int_half_modulus.
       move ? : (bits_per_int it - 1) => k.
-      have ? : 0 ≤ k.
-      { suff : bits_per_int it > 0 by lia. by apply: bits_per_int_gt_0. }
-      have Hb : ∀ n, -2^k ≤ n ≤ 2^k - 1 ↔
-        ∀ l, k ≤ l → Z.testbit n l = bool_decide (n < 0)
-        by intros; rewrite -bounded_iff_bits; lia.
+      have Hb : ∀ n, -2^k ≤ n ≤ 2^k - 1 ↔ ∀ l, k ≤ l → Z.testbit n l = bool_decide (n < 0).
+      { move => ?. rewrite -Z_bounded_iff_bits; lia. }
       move => /Hb Hn1 /Hb Hn2.
       apply Hb => l Hl.
       by rewrite Htestbit Hsign Hn1 ?Hn2.
     - rewrite /int_modulus.
       move ? : (bits_per_int it) => k.
-      have ? : 0 ≤ k.
-      { suff : bits_per_int it > 0 by lia. by apply: bits_per_int_gt_0. }
-      have Hb : ∀ n, 0 ≤ n → n ≤ 2^k - 1 ↔
-        ∀ l, k ≤ l → Z.testbit n l = bool_decide (n < 0)
-        by intros; rewrite bool_decide_false -?pos_bounded_iff_bits; lia.
+      have Hb : ∀ n, 0 ≤ n → n ≤ 2^k - 1 ↔ ∀ l, k ≤ l → Z.testbit n l = bool_decide (n < 0).
+      { move => ??. rewrite bool_decide_false -?Z_bounded_iff_bits_nonneg; lia. }
       move => [Hn1 /Hb HN1] [Hn2 /Hb HN2].
       have Hn := Hnonneg Hn1 Hn2.
       split; first done.
